theories/L6_PCPS/Heap/closure_conversion_correct.v
@@ -549,43 +549,7 @@ Module ClosureConversionCorrect (H : Heap).
     intros Hvar. rewrite Union_Same_set. reflexivity.
     eapply project_vars_In_Union.
     eassumption.
-  Qed.
-
-  Definition cc_approx_heap (S : Ensemble loc) k j IP P b d (H1 H2 : heap block) :=
-    forall (l : loc), l \in S ->
-                 Res (Loc l, H1) ≺ ^ (k; j; IP; P; b; d) Res (Loc (b l), H2).
-
-  Notation "S |- H1 ≼ ^ ( k ; j ; IP ; P ; b ; d ) H2" :=
-    (cc_approx_heap S k j IP P b d H1 H2)
-      (at level 70, no associativity).
-
-  (* move *)
-  Lemma Ensemble_ind (P : Ensemble var -> Prop) {_ : Proper (Same_set _ ==> iff) P} :
-    P (Empty_set _) ->
-    (forall x S {_ : ToMSet S}, ~ x \in S -> P S -> P (x |: S)) ->
-    (forall S {_ : ToMSet S}, P S).
-  Proof.
-    intros Hbase IH S HS.
-    eapply H. eapply HS.
-    eapply PS_ind with (S := mset).
-    - intros x y Heq. eapply H.
-      unfold FromSet. rewrite Heq. reflexivity.
-    - rewrite FromSet_empty. eassumption.
-    - intros z S1 Hnin HP.
-      rewrite FromSet_add. eapply IH; try eassumption.
-      econstructor. reflexivity.
-      intros Hc. eapply Hnin. unfold FromSet, FromList, In in Hc.
-      simpl in Hc. eapply In_InA in Hc. eapply PS.elements_spec1 in Hc.
-      eassumption. eauto with typeclass_instances.
-  Qed.
-
-  Definition injective_subdomain' {A B} P (f : A -> option B) :=
-    forall x x' v, In _ P x -> In _ P x' -> f x = Some v -> f x' = Some v -> x = x'.
-
-  Require Import Permutation.
-
-  (* TODO move *)
- 
+  Qed. 
     
   Lemma size_reachable_leq S1 `{HS1 : ToMSet S1}  S2 `{HS2 : ToMSet S2}
         H1 H2 k GIP GP b d :
@@ -600,24 +564,38 @@ Module ClosureConversionCorrect (H : Heap).
   Proof with (now eauto with Ensembles_DB).
     assert (HS1' := HS1).
     revert HS1 S2 HS2.
+    set (P := (fun S1 => 
+                 forall (HS1 : ToMSet S1) (S2 : Ensemble positive) (HS2 : ToMSet S2),
+                   (forall j, S1 |- H1 ≼ ^ (k; j; GIP; GP; b; d) H2) ->
+                   S2 <--> image b S1 :|: image' d S1 ->
+                   injective_subdomain S1 b ->
+                   injective_subdomain' S1 d ->
+                   Disjoint _ (image b S1) (image' d S1) ->
+                   size_with_measure_filter size_val S1 H1 <=
+                   size_with_measure_filter size_val S2 H2 <=
+                   (size_with_measure_filter size_val S1 H1) * (1 + (max_vars_heap H1))
+              )). 
+    assert (HP : Proper (Same_set var ==> iff) P).
+    { intros S1' S2' Hseq. unfold P.
+      split; intros.
+
+      assert (HMS1' : ToMSet S1').
+      { eapply ToMSet_Same_set. symmetry. eassumption. eassumption. }
+      erewrite <- (@HL.size_with_measure_Same_set _ _ _ _ _ _ _ Hseq).
+      eapply H; try eassumption; repeat setoid_rewrite Hseq at 1; try eassumption.
+
+      assert (HMS2' : ToMSet S2').
+      { eapply ToMSet_Same_set; eassumption. }
+      erewrite (@HL.size_with_measure_Same_set _ _ _ _ _ _ _ Hseq).
+      eapply H; try eassumption; repeat setoid_rewrite <- Hseq at 1; try eassumption. }
     
-    eapply (Ensemble_ind (fun S1 => 
-                            forall (HS1 : ToMSet S1) (S2 : Ensemble positive) (HS2 : ToMSet S2),
-                              (forall j, S1 |- H1 ≼ ^ (k; j; GIP; GP; b; d) H2) ->
-                              S2 <--> image b S1 :|: image' d S1 ->
-                              injective_subdomain S1 b ->
-                              injective_subdomain' S1 d ->
-                              Disjoint _ (image b S1) (image' d S1) ->
-                              size_with_measure_filter size_val S1 H1 <=
-                              size_with_measure_filter size_val S2 H2 <=
-                              (size_with_measure_filter size_val S1 H1) * (1 + (max_vars_heap H1))
-                         )); [| | eassumption ].
+    eapply (@Ensemble_ind P HP); [| | eassumption ].
     - intros HS1 S2 HS2 Hcc Heq Hinj1 Hinj2 HD.
-      rewrite !size_with_measure_filter_Empty_set.
+      rewrite !HL.size_with_measure_filter_Empty_set.
       rewrite image_Empty_set, image'_Empty_set in Heq.
       rewrite Union_Empty_set_neut_r in Heq.
       simpl. erewrite (@HL.size_with_measure_Same_set _ _ _ _ _ _ _ Heq).
-      rewrite size_with_measure_filter_Empty_set. omega.
+      rewrite HL.size_with_measure_filter_Empty_set. omega.
     - intros x S1' HS Hnin IHS HS1 S2 HS2 Hheap Heq Hinj1 Hinj2 HD.
       rewrite image_Union, image'_Union, image_Singleton in Heq.
       unfold mset.
@@ -625,28 +603,74 @@ Module ClosureConversionCorrect (H : Heap).
       assert (Hseq : S2 <--> b x |: (image' d [set x]) :|: (S2 \\ (b x |: (image' d [set x])))). 
       { eapply Union_Setminus_Same_set.
         eapply Decidable_Union. eapply DecidableSingleton_positive.
-        admit. 
+        
+        destruct (d x) eqn:Heqd.
+        eapply Decidable_Same_set. 
+        erewrite image'_Singleton_Some. reflexivity. eassumption.
+        now eauto with typeclass_instances.
+
+        eapply Decidable_Same_set. 
+        erewrite image'_Singleton_None. reflexivity. eassumption.
+        now eauto with typeclass_instances.
+
         rewrite Heq. now eauto with Ensembles_DB. }
-      assert (HS2' : ToMSet (S2 \\ (b x |: image' d [set x]))) by now eauto with typeclass_instances.
+
+      assert (HS2' : ToMSet (S2 \\ (b x |: image' d [set x])))
+        by now eauto with typeclass_instances.
       
       specialize (IHS HS1'' _ HS2').
-      
-      assert (Hcc : (forall j, Res (Loc x, H1) ≺ ^ (k ; j ; GIP ; GP ; b ; d) Res (Loc (b x), H2))). 
+       
+      assert (Hcc : (forall j, Res (Loc x, H1) ≺ ^ (k ; j ; GIP ; GP ; b ; d) Res (Loc (b x), H2))).
       { intros j; eapply Hheap. now left. }
       
+      assert (Hseq' : b x |: image b S1' :|: (image' d [set x] :|: image' d S1') <-->
+                        b x |: image' d [set x] :|: (image b S1' :|: image' d S1')).
+
+      { rewrite <- Union_assoc, (Union_assoc (image b S1'))... }
+      rewrite Hseq' in Heq.
+
+      assert (Hseq'' :  S2 \\ (b x |: image' d [set x]) <--> image b S1' :|: image' d S1').
+      { rewrite Heq. rewrite Setminus_Union_distr.
+        rewrite Setminus_Same_set_Empty_set. rewrite Union_Empty_set_neut_l.
+        rewrite Setminus_Disjoint. reflexivity.
+        rewrite image_Union, image'_Union, image_Singleton in HD.
+        
+        eapply Union_Disjoint_l; eapply Union_Disjoint_r. 
+        + eapply Disjoint_Singleton_r. intros [y [Hin Hc]].
+          eapply Hinj1 in Hc. now subst; eauto.
+          now right. now left.
+        + eapply Disjoint_Included; [| | eassumption ]...
+        + eapply Disjoint_sym. eapply Disjoint_Included; [| | eassumption ]...
+        + constructor. intros l1. intros [l2 [y [Hin1 Hc1]] [y' [Hin2 Hc2]]].
+          inv Hin2. eapply Hinj2 in Hc2. eapply Hc2 in Hc1. now subst; eauto.
+          now left. now right. }
+
       destruct (get x H1) as [v | ] eqn:Hget1;
         [| destruct (Hcc 0) as [_ Hcc']; rewrite Hget1 in Hcc'; contradiction ]. 
       
-      erewrite (HL.size_with_measure_Same_set _ _ _ _ H2 Heq).
-      erewrite HL.size_with_measure_filter_add_In; try eassumption.
-      erewrite size_with_measure_filter_Union.
-      + admit.
-      + constructor.
-        intros l [l1 Hc1 Hc2]. eapply HD. constructor.
-        rewrite image_Union, image_Singleton. eassumption.
-        rewrite image'_Union. eassumption.
+      erewrite (HL.size_with_measure_Same_set _ _ _ _ H2 Hseq).
+      erewrite HL.size_with_measure_filter_add_In; try eassumption. 
+      erewrite HL.size_with_measure_filter_Union.
+      + assert (Hleq :
+                  size_with_measure_filter size_val S1' H1 <=
+                  size_with_measure_filter size_val (S2 \\ (b x |: image' d [set x]))
+                                           H2 <=
+                  size_with_measure_filter size_val S1' H1 * (1 + max_vars_heap H1)).
+        { eapply IHS.
+          - intros j. eapply cc_approx_heap_antimon; [| now eapply Hheap; eauto ]...
+          - eassumption.
+          - eapply injective_subdomain_antimon; [ eassumption |]...
+          - eapply injective_subdomain'_antimon; [ eassumption |]...
+          - eapply Disjoint_Included; [| | eassumption ]... }
+        assert (Hleqv : size_val v <=
+                        size_with_measure_filter size_val (b x |: image' d [set x]) H2 <=
+                        (size_val v) *  (1 + max_vars_heap H1)).
+        { admit. } 
+        split. omega.
+        rewrite Nat.mul_add_distr_r. omega. 
+      + eapply Disjoint_Setminus_r. reflexivity.
+  Admitted. 
         
-    
 
   (* Lemma image_FV GI GP k β H1 rho1 H2 rho2 Scope `{Decidable _ Scope} FVs Γ c : *)
   (*   (forall j, (H1, rho1) ⋞ ^ (Scope ; k ; j ; GI ; GP ; β; d) (H2, rho2)) -> *)
